Test/sequences/intseq.bpl
@@ -1,22 +1,22 @@
 // RUN: %boogie "%s" > "%t"
 // RUN: %diff "%s.expect" "%t"
 
-type {:builtin "(Seq Int)"} IntSeq;
-function {:builtin "(as seq.empty (Seq Int))"} EmptyIntSeq(): IntSeq;
-function {:builtin "seq.len"} IntSeqLen(s: IntSeq): int;
-function {:builtin "seq.++"} IntSeqConcat(s1: IntSeq, s2:IntSeq): IntSeq;
-function {:builtin "seq.unit"} IntSeqUnit(i: int): IntSeq;
-function {:builtin "seq.nth"} IntSeqNth(s: IntSeq, i: int): int;
-function {:builtin "seq.extract"} IntSeqExtract(s: IntSeq, pos: int, len: int): IntSeq;
+type {:builtin "Seq"} Seq _;
+function {:builtin "seq.empty"} Seq_Empty_int(): Seq int;
+function {:builtin "seq.len"} Seq_Len_int(a: Seq int): int;
+function {:builtin "seq.++"} Seq_Concat_int(a: Seq int, b: Seq int): Seq int;
+function {:builtin "seq.unit"} Seq_Unit_int(v: int): Seq int;
+function {:builtin "seq.nth"} Seq_Nth_int(a: Seq int, i: int): int;
+function {:builtin "seq.extract"} Seq_Extract_int(a: Seq int, pos: int, length: int): Seq int;
 
 procedure test()
 {
-  var s: IntSeq;
+  var s: Seq int;
 
-  s := IntSeqConcat(EmptyIntSeq(), IntSeqUnit(0));
-  s := IntSeqConcat(s, IntSeqUnit(1));
-  s := IntSeqConcat(s, IntSeqUnit(2));
-  assert IntSeqLen(s) == 3;
-  assert IntSeqExtract(s, 1, 2) == IntSeqConcat(IntSeqUnit(1), IntSeqUnit(2));
-  assert IntSeqNth(s, 1) == 1;
+  s := Seq_Concat_int(Seq_Empty_int(), Seq_Unit_int(0));
+  s := Seq_Concat_int(s, Seq_Unit_int(1));
+  s := Seq_Concat_int(s, Seq_Unit_int(2));
+  assert Seq_Len_int(s) == 3;
+  assert Seq_Extract_int(s, 1, 2) == Seq_Concat_int(Seq_Unit_int(1), Seq_Unit_int(2));
+  assert Seq_Nth_int(s, 1) == 1;
 }
