Test/sequences/intseq_datatype.bpl
@@ -6,42 +6,42 @@ type {:datatype} Value;
 function {:constructor} Integer(i: int): Value;
 function {:constructor} Vector(v: ValueArray): Value;
 
-type {:builtin "(Seq T@Value)"} ValueSeq;
-function {:builtin "(as seq.empty (Seq T@Value))"} EmptyValueSeq(): ValueSeq;
-function {:builtin "seq.len"} ValueSeqLen(a: ValueSeq): int;
-function {:builtin "seq.++"} ValueSeqConcat(a: ValueSeq, b:ValueSeq): ValueSeq;
-function {:builtin "seq.unit"} ValueSeqUnit(v: Value): ValueSeq;
-function {:builtin "seq.nth"} ValueSeqNth(a: ValueSeq, i: int): Value;
-function {:builtin "seq.extract"} ValueSeqExtract(a: ValueSeq, pos: int, length: int): ValueSeq;
+type {:builtin "Seq"} Seq _;
+function {:builtin "seq.empty"} Seq_Empty_Value(): Seq Value;
+function {:builtin "seq.len"} Seq_Len_Value(a: Seq Value): int;
+function {:builtin "seq.++"} Seq_Concat_Value(a: Seq Value, b: Seq Value): Seq Value;
+function {:builtin "seq.unit"} Seq_Unit_Value(v: Value): Seq Value;
+function {:builtin "seq.nth"} Seq_Nth_Value(a: Seq Value, i: int): Value;
+function {:builtin "seq.extract"} Seq_Extract_Value(a: Seq Value, pos: int, length: int): Seq Value;
 
-type {:datatype} {:dependson "Value"} ValueArray;
-function {:constructor} ValueArray(v: ValueSeq): ValueArray;
+type {:datatype} ValueArray;
+function {:constructor} ValueArray(v: Seq Value): ValueArray;
 function {:inline} EmptyValueArray(): ValueArray {
-    ValueArray(EmptyValueSeq())
+    ValueArray(Seq_Empty_Value())
 }
 function {:inline} AddValueArray(a: ValueArray, v: Value): ValueArray {
-    ValueArray(ValueSeqConcat(v#ValueArray(a),ValueSeqUnit(v)))
+    ValueArray(Seq_Concat_Value(v#ValueArray(a),Seq_Unit_Value(v)))
 }
 function {:inline} RemoveValueArray(a: ValueArray): ValueArray {
-    ValueArray(ValueSeqExtract(v#ValueArray(a), 0, ValueSeqLen(v#ValueArray(a)) - 1))
+    ValueArray(Seq_Extract_Value(v#ValueArray(a), 0, Seq_Len_Value(v#ValueArray(a)) - 1))
 }
 function {:inline} ConcatValueArray(a1: ValueArray, a2: ValueArray): ValueArray {
-    ValueArray(ValueSeqConcat(v#ValueArray(a1), v#ValueArray(a2)))
+    ValueArray(Seq_Concat_Value(v#ValueArray(a1), v#ValueArray(a2)))
 }
 function {:inline} IsEmpty(a: ValueArray): bool {
-    ValueSeqLen(v#ValueArray(a)) == 0
+    Seq_Len_Value(v#ValueArray(a)) == 0
 }
 function {:inline} LenValueArray(a: ValueArray): int {
-    ValueSeqLen(v#ValueArray(a))
+    Seq_Len_Value(v#ValueArray(a))
 }
 function {:inline} ValueArrayAt(a: ValueArray, i: int): Value {
-    ValueSeqNth(v#ValueArray(a), i)
+    Seq_Nth_Value(v#ValueArray(a), i)
 }
 
 procedure test()
 {
   var s: ValueArray;
-  
+
   s := EmptyValueArray();
   assert IsEmpty(s);
   s := AddValueArray(s, Integer(0));
