Test/sequences/intseq_datatype_lib.bpl
@@ -1,0 +1,49 @@
+// RUN: %boogie -lib "%s" > "%t"
+// RUN: %diff "%s.expect" "%t"
+
+type {:datatype} Value;
+
+function {:constructor} Integer(i: int): Value;
+function {:constructor} Vector(v: Array Value): Value;
+
+type {:datatype} Array _;
+function {:constructor} Array<T>(v: Seq T): Array T;
+function {:inline} EmptyArray<T>(): Array T {
+    Array(Seq_Empty())
+}
+function {:inline} AddArray<T>(a: Array T, v: T): Array T {
+    Array(Seq_Concat(v#Array(a), Seq_Unit(v)))
+}
+function {:inline} RemoveArray<T>(a: Array T): Array T {
+    Array(Seq_Extract(v#Array(a), 0, Seq_Len(v#Array(a)) - 1))
+}
+function {:inline} ConcatArray<T>(a1: Array T, a2: Array T): Array T {
+    Array(Seq_Concat(v#Array(a1), v#Array(a2)))
+}
+function {:inline} IsEmpty<T>(a: Array T): bool {
+    Seq_Len(v#Array(a)) == 0
+}
+function {:inline} LenArray<T>(a: Array T): int {
+    Seq_Len(v#Array(a))
+}
+function {:inline} ArrayAt<T>(a: Array T, i: int): T {
+    Seq_Nth(v#Array(a), i)
+}
+
+procedure test()
+{
+  var s: Array Value;
+
+  s := EmptyArray();
+  assert IsEmpty(s);
+  s := AddArray(s, Integer(0));
+  s := AddArray(s, Integer(1));
+  s := AddArray(s, Integer(2));
+  assert LenArray(s) == 3;
+  assert ArrayAt(s, 1) == Integer(1);
+  s := RemoveArray(s);
+  assert(LenArray(s)) == 2;
+  s := ConcatArray(s, s);
+  assert LenArray(s) == 4;
+  assert ArrayAt(s, 3) == Integer(1);
+}
