Test/sequences/intseq_lib.bpl
@@ -1,0 +1,14 @@
+// RUN: %boogie -lib "%s" > "%t"
+// RUN: %diff "%s.expect" "%t"
+
+procedure test()
+{
+  var s: Seq int;
+
+  s := Seq_Concat(Seq_Empty(), Seq_Unit(0));
+  s := Seq_Concat(s, Seq_Unit(1));
+  s := Seq_Concat(s, Seq_Unit(2));
+  assert Seq_Len(s) == 3;
+  assert Seq_Extract(s, 1, 2) == Seq_Concat(Seq_Unit(1), Seq_Unit(2));
+  assert Seq_Nth(s, 1) == 1;
+}
